Add swap operator and sketch infra for it. Update several mistakes in LTS
This is after meeting Serguei Lenglet, who showed us his proof (for pi calculus without sums) and highlighted some mistakes we had.

theories/Pi_Instance.v
@@ -46,6 +46,8 @@ Open Scope subst_scope.
 Notation "⋅" := ids.
 Notation "tm ⟨ r ⟩" := (ren2 ids r tm) (at level 20).
 
+Arguments core.funcomp _ _ _/.
+
 (*Coercion makes the specification of 'cst' and 'bvar' useless, then simplify the notation *)
 Coercion cst : Value >-> Data.
 Coercion var_Data : nat >-> Data.
@@ -131,16 +133,16 @@ induction n.
 - intros. simpl. now rewrite IHn.
 Qed.
 
+Definition injective (σ : nat -> nat) :=
+  forall x y, σ x = σ y -> x = y.
 
-Definition swap_two p :=
-  ren_proc ids (fun x => match x with 0 => S 0 | S 0 => 0 | n => n end) p.
-(* have this automatically unfold *)
-Arguments swap_two / _.
+Definition swap : nat -> nat := 1 .: (0 .: (shift >> shift >> ids)).
 
-(* Lemma swap_two_example : exists p, p =
-  swap_two
-   (0 ? (0 ! var_Data 0 • ①) ‖ (1 ! var_Data 1 • (1 ? (1 ! var_Data 1 • ①)))).
-   unfold swap_two. asimpl. unfold core.funcomp. *)
+Lemma swap_involutive : forall x, (swap >> swap) x = ids x.
+Proof.
+  intros [|[|x]]; reflexivity.
+Qed.
+
 
 Reserved Notation "p ≡ q" (at level 70).
 Inductive cgr_step : proc -> proc -> Prop :=
@@ -195,8 +197,8 @@ Inductive cgr_step : proc -> proc -> Prop :=
     (g p1) ≡ (g q1) -> 
     (p1 + p2) ≡ (q1 + p2)
 
-(* | cgr_nu_nu_step : forall p,
-    (ν ν p) ≡ (ν ν (swap_two p)) *)
+| cgr_nu_nu_step : forall p,
+    (ν ν p) ≡ (ν ν (p ⟨swap⟩))
 | cgr_res_nil_step :
     (ν 𝟘) ≡ 𝟘
 | cgr_res_nil_rev_step :
@@ -228,12 +230,21 @@ where "p ≡ q" := (cgr_step p q).
   | If C Then p Else q => S (size p + size q)
 end. *)
 
+
+(* Require functional extensionality *)
+
+From Coq Require Import FunctionalExtensionality.
+
 (* The relation ≡ is an reflexive*)
 #[global] Instance cgr_refl_step_is_refl : Reflexive cgr_step.
 Proof. intro. apply cgr_refl_step. Qed.
 (* The relation ≡ is symmetric*)
 #[global] Instance cgr_symm_step : Symmetric cgr_step.
 Proof. intros p q hcgr. induction hcgr; try solve [constructor; try exact IHhcgr].
+- assert (p = p ⟨swap⟩ ⟨swap⟩).
+  {assert (Hext : (swap >> swap) = ids) by apply functional_extensionality, swap_involutive.
+  asimpl. simpl. rewrite Hext. asimpl. reflexivity. }
+  rewrite H at 2. apply cgr_nu_nu_step.
 Qed.
 (* - assert (swap_two (swap_two p) = p).
   + unfold swap_two. admit.
@@ -344,6 +355,10 @@ intros. dependent induction H.
 - constructor. apply cgr_res_step. exact H.
 - eauto with cgr_eq.
 Qed.
+Lemma cgr_nu_nu : forall p, (ν ν p) ≡* (ν ν (p ⟨swap⟩)).
+Proof.
+intros p. constructor. apply cgr_nu_nu_step.
+Qed.
 Lemma cgr_res_nil : 𝟘 ≡* (ν 𝟘).
 Proof.
 constructor. exact cgr_res_nil_rev_step.
@@ -447,7 +462,6 @@ Qed. *)
 
 (* The old Congruence lemmas can now be restated using Autosubst's help.
    This still requires some technical work and lemmas on substitutions. *)
-Arguments core.funcomp _ _ _/.
 
 Lemma permute_subst : forall sp s Q,
   (⇑ Q) [(up_Data_proc sp); (up_Data_Data s)]
@@ -468,10 +482,11 @@ intros sp' sp Hp s' s Hs q1 q2 Hq.
 induction Hq as [p q base_case | p r q transitivity_case].
 - subst. revert sp s. induction base_case; intros; try solve [asimpl; auto with cgr].
   + asimpl. apply cgr_choice. apply IHbase_case.
+  + admit. (* Swap case *)
   + unfold subst2. simpl. rewrite permute_subst. exact (cgr_scope _ _).
   + unfold subst2. simpl. rewrite permute_subst. exact (cgr_scope_rev _ _).
 - subst. now rewrite IHtransitivity_case.
-Qed.
+Admitted.
 
 Instance SubstProper' : Proper (eq_up_to_cgr ==> eq ==> eq ==> cgr) subst2.
 Proof.
@@ -511,10 +526,11 @@ induction Hq as [p q base_case | p r q transitivity_case].
 - subst. revert sp s. induction base_case; intros; try solve [asimpl; auto with cgr].
   (* + simpl. unfold subst2. simpl. substify. simpl. Set Printing All. *)
   + asimpl. apply cgr_choice. apply IHbase_case.
+  + asimpl. simpl. admit. (* Swap case *)
   + unfold ren2. simpl. rewrite permute_ren. exact (cgr_scope _ _).
   + unfold ren2. simpl. rewrite permute_ren. exact (cgr_scope_rev _ _).
 - subst. now rewrite IHtransitivity_case.
-Qed.
+Admitted.
 
 Instance NewsProper : Proper (eq ==> cgr ==> cgr) νs.
 Proof.
@@ -761,6 +777,7 @@ Definition is_bound_out (a:Act) : bool :=
   end.
 
 Notation "a '⇑?' p" := (if is_bound_out a then ⇑ p else p) (at level 20).
+Notation "a '?↔' p" := (if is_bound_out a then p ⟨swap⟩ else p) (at level 20).
 
 (* The Labelled Transition System (LTS-transition) *)
 Inductive lts : proc-> Act -> proc -> Prop :=
@@ -793,15 +810,15 @@ Inductive lts : proc-> Act -> proc -> Prop :=
 (* Scoped rules *)
 | lts_close_l : forall {c p1 p2 q1 q2},
     lts p1 (BoundOut c) p2 ->      (* this term is an "open" term, (see the lts_open rule) *)
-    lts q1 (ActIn (c ⋉ 0)) q2 ->  (* while this one is a "closed" term *)
+    lts (⇑ q1) (ActIn (c ⋉ 0)) q2 ->  (* while this one is a "closed" term *)
     lts (p1 ‖ q1) τ (ν (p2 ‖ q2))   (* so whe should shift q2 here. This corresponds to cgr_scope (scope extrusion) *)
 | lts_close_r : forall {c p1 p2 q1 q2},
     lts q1 (BoundOut c) q2 ->
-    lts p1 (ActIn (c ⋉ 0)) p2 ->
+    lts (⇑ p1) (ActIn (c ⋉ 0)) p2 ->
     lts (p1 ‖ q1) τ (ν (p2 ‖ q2))
 | lts_res : forall {p q α},
     lts p (⇑ α) q ->
-    lts (ν p) α (ν q)
+    lts (ν p) α (ν (α ?↔ q ))
                       (* only α needs to shift here!! (both chan and value).
                          as a consequence, the channel in α can never be 0 (giving the condition in paper)
                          as in onther places: we started with an "open" value, that's why we add a flat ν *)
@@ -912,7 +929,7 @@ dependent induction Transition; try destruct (IHTransition c v eq_refl) as (P1 &
 - destruct (IHTransition (⇑ c) (⇑ v) eq_refl) as (P1 & G & R & n & cn & vn & H0 & H1 & H3 & H2).
     exists P1, G, R, (S n), cn, vn. do 3 (try split).
   + now rewrite H0.
-  + now rewrite H1.
+  + simpl. now rewrite H1.
   + rewrite H3. simpl. now rewrite shift_in_nvars.
   + not_a_guard.
 - destruct n.
@@ -1221,8 +1238,8 @@ Proof with (subst; eauto with lts cgr).
       (* lts_close_l *)
       * dependent destruction l2.
         -- eexists (ν ((p2 ‖ p0) ‖ r)). split.
-            ++ eapply lts_close_l.
-            ++ reflexivity.
+            ++ admit.
+            ++ admit.
         -- eexists. split.
            ++ eapply (lts_close_l _ _).
            ++ reflexivity.
@@ -1299,9 +1316,7 @@ Proof with (subst; eauto with lts cgr).
         eexists. split.
         ** apply (lts_close_l H0 l2).
         ** now rewrite H1.
-      * destruct (IHcgr_step p2 _ l2) as [x [H0 H1]]. eexists. split.
-        ** apply (lts_close_r l1 H0).
-        ** unfold shift_op, Shiftable_proc. now rewrite H1.
+      * admit. (* The issue with inductive hypothesis that Serguei was talking about *)
       * destruct (IHcgr_step p2 α l) as [x H0]. destruct H0...
       * eexists (α ⇑? p ‖ q2). split.
         -- apply lts_parR...
